Reimplemented F* conversion modules

fstar/Zen.UInt64.Conversion.fst
@@ -1,7 +1,8 @@
 module Zen.UInt64.Conversion
 
-module UInt64 = FStar.Int64
-open            FStar.UInt64
+open FStar.UInt64
+
+module Int64  = FStar.Int64
 module UInt32 = FStar.UInt32
 module UInt8  = FStar.UInt8
 
@@ -14,14 +15,14 @@ abstract let fromUInt32 x = uint_to_t (UInt32.v x)
 abstract val fromUInt8 : x:UInt8.t {fits (UInt8.v x)} -> t
 abstract let fromUInt8 x = uint_to_t (UInt8.v x)
 
-abstract val fromInt64opt : x:Int64.t -> option t
-abstract let fromInt64opt x = if fits (Int64.v x) then Some <| uint_to_t (Int64.v x) else None
+abstract val tryFromInt64 : x:Int64.t -> option t
+abstract let tryFromInt64 x = if fits (Int64.v x) then Some <| uint_to_t (Int64.v x) else None
 
-abstract val fromUInt32opt : x:UInt32.t -> option t
-abstract let fromUInt32opt x = if fits (UInt32.v x) then Some <| uint_to_t (UInt32.v x) else None
+abstract val tryFromUInt32 : x:UInt32.t -> option t
+abstract let tryFromUInt32 x = if fits (UInt32.v x) then Some <| uint_to_t (UInt32.v x) else None
 
-abstract val fromUInt8opt : x:UInt8.t -> option t
-abstract let fromUInt8opt x = if fits (UInt8.v x) then Some <| uint_to_t (UInt8.v x) else None
+abstract val tryFromUInt8 : x:UInt8.t -> option t
+abstract let tryFromUInt8 x = if fits (UInt8.v x) then Some <| uint_to_t (UInt8.v x) else None
 
 abstract val toInt64 : x:t {Int64.fits (v x)} -> Int64.t
 abstract let toInt64 x = Int64.int_to_t (v x)
@@ -32,59 +33,59 @@ abstract let toUInt32 x = UInt32.uint_to_t (v x)
 abstract val toUInt8 : x:t {UInt8.fits (v x)} -> UInt8.t
 abstract let toUInt8 x = UInt8.uint_to_t (v x)
 
-abstract val toInt64opt : x:t -> option Int64.t
-abstract let toInt64opt x = if Int64.fits (v x) then Some <| Int64.int_to_t (v x) else None
+abstract val tryToInt64 : x:t -> option Int64.t
+abstract let tryToInt64 x = if Int64.fits (v x) then Some <| Int64.int_to_t (v x) else None
 
-abstract val toUInt32opt : x:t -> option UInt32.t
-abstract let toUInt32opt x = if UInt32.fits (v x) then Some <| UInt32.uint_to_t (v x) else None
+abstract val tryToUInt32 : x:t -> option UInt32.t
+abstract let tryToUInt32 x = if UInt32.fits (v x) then Some <| UInt32.uint_to_t (v x) else None
 
-abstract val toUInt8opt : x:t -> option UInt8.t
-abstract let toUInt8opt x = if UInt8.fits (v x) then Some <| UInt8.uint_to_t (v x) else None
+abstract val tryToUInt8 : x:t -> option UInt8.t
+abstract let tryToUInt8 x = if UInt8.fits (v x) then Some <| UInt8.uint_to_t (v x) else None
 
-val v_invariant_fromInt64 : x:Int64.t {fits (Int64.v x)} -> Lemma
-    (ensures (Int64.v x == v (fromInt64 x)))
-let v_invariant_fromInt64 x = ()
+val v_fromInt64 : x:Int64.t {fits (Int64.v x)} -> Lemma
+    (Int64.v x == v (fromInt64 x))
+let v_fromInt64 x = ()
 
-val v_invariant_fromUInt32 : x:UInt32.t {fits (UInt32.v x)} -> Lemma
-    (ensures (UInt32.v x == v (fromUInt32 x)))
-let v_invariant_fromUInt32 x = ()
+val v_fromUInt32 : x:UInt32.t {fits (UInt32.v x)} -> Lemma
+    (UInt32.v x == v (fromUInt32 x))
+let v_fromUInt32 x = ()
 
-val v_invariant_fromUInt8 : x:UInt8.t {fits (UInt8.v x)} -> Lemma
-    (ensures (UInt8.v x == v (fromUInt8 x)))
-let v_invariant_fromUInt8 x = ()
+val v_fromUInt8 : x:UInt8.t {fits (UInt8.v x)} -> Lemma
+    (UInt8.v x == v (fromUInt8 x))
+let v_fromUInt8 x = ()
 
-val v_invariant_toInt64 : x:t {Int64.fits (v x)} -> Lemma
-    (ensures (Int64.v (toInt64 x) == v x))
-let v_invariant_toInt64 x = ()
+val v_toInt64 : x:t {Int64.fits (v x)} -> Lemma
+    (Int64.v (toInt64 x) == v x)
+let v_toInt64 x = ()
 
-val v_invariant_toUInt32 : x:t {UInt32.fits (v x)} -> Lemma
-    (ensures (UInt32.v (toUInt32 x) == v x))
-let v_invariant_toUInt32 x = ()
+val v_toUInt32 : x:t {UInt32.fits (v x)} -> Lemma
+    (UInt32.v (toUInt32 x) == v x)
+let v_toUInt32 x = ()
 
-val v_invariant_toUInt8 : x:t {UInt8.fits (v x)} -> Lemma
-    (ensures (UInt8.v (toUInt8 x) == v x))
-let v_invariant_toUInt8 x = ()
+val v_toUInt8 : x:t {UInt8.fits (v x)} -> Lemma
+    (UInt8.v (toUInt8 x) == v x)
+let v_toUInt8 x = ()
 
-val inbounds_some_fromInt64opt : x:Int64.t {fits (Int64.v x)} -> Lemma
-    (Some? (fromInt64opt x))
-let inbounds_some_fromInt64opt x = ()
+val v_tryFromInt64 : x:Int64.t -> Lemma
+    (fits (Int64.v x) ==> Int64.v x == v (Some?.v (tryFromInt64 x)))
+let v_tryFromInt64 x = ()
 
-val inbounds_some_fromUInt32opt : x:UInt32.t {fits (UInt32.v x)} -> Lemma
-    (Some? (fromUInt32opt x))
-let inbounds_some_fromUInt32opt x = ()
+val v_tryFromUInt32 : x:UInt32.t -> Lemma
+    (fits (UInt32.v x) ==> UInt32.v x == v (Some?.v (tryFromUInt32 x)))
+let v_tryFromUInt32 x = ()
 
-val inbounds_some_fromUInt8opt : x:UInt8.t {fits (UInt8.v x)} -> Lemma
-    (Some? (fromUInt8opt x))
-let inbounds_some_fromUInt8opt x = ()
+val v_tryFromUInt8 : x:UInt8.t -> Lemma
+    (fits (UInt8.v x) ==> UInt8.v x == v (Some?.v (tryFromUInt8 x)))
+let v_tryFromUInt8 x = ()
 
-val inbounds_some_toInt64opt : x:t {Int64.fits (v x)} -> Lemma
-    (Some? (toInt64opt x))
-let inbounds_some_toInt64opt x = ()
+val v_tryToInt64 : x:t -> Lemma
+    (Int64.fits (v x) ==> Int64.v (Some?.v (tryToInt64 x)) == v x)
+let v_tryToInt64 x = ()
 
-val inbounds_some_toUInt32opt : x:t {UInt32.fits (v x)} -> Lemma
-    (Some? (toUInt32opt x))
-let inbounds_some_toUInt32opt x = ()
+val v_tryToUInt32 : x:t -> Lemma
+    (UInt32.fits (v x) ==> UInt32.v (Some?.v (tryToUInt32 x)) == v x)
+let v_tryToUInt32 x = ()
 
-val inbounds_some_toUInt8opt : x:t {UInt8.fits (v x)} -> Lemma
-    (Some? (toUInt8opt x))
-let inbounds_some_toUInt8opt x = ()
+val v_tryToUInt8 : x:t -> Lemma
+    (UInt8.fits (v x) ==> UInt8.v (Some?.v (tryToUInt8 x)) == v x)
+let v_tryToUInt8 x = ()
